upgrade to latest freezable buffers now in F* master

src/lowparse/LowParseExampleMono.fst
@@ -1,6 +1,6 @@
 module LowParseExampleMono
 include LowParse.MLow.Base
-open LowStar.FreezableBuffer
+open LowStar.PrefixFreezableBuffer
 
 module U32 = FStar.UInt32
 module U8 = FStar.UInt8
@@ -17,44 +17,45 @@ let compl
 : GTot Type0
 = U32.v pos >= 4 /\
   Seq.length x >= 4 /\ (
-  let len = get_w x in
+  let len = frozen_until x in
   len >= 4 /\ len <= Seq.length x /\
   U32.v pos' <= len
   )
 
 inline_for_extraction
-type fslice = (s: slice freezable_preorder freezable_preorder {
+type slice = (s: slice prefix_freezable_preorder prefix_freezable_preorder {
   B.length s.base >= 4 /\
-  B.witnessed s.base (w_pred 4)
+  B.witnessed s.base (frozen_until_at_least 4)
 })
 
 inline_for_extraction
-let make_fslice
-  (b: fbuffer)
+let make_slice
+  (b: buffer)
   (len: U32.t { U32.v len == B.length b } )
-: Tot fslice
+: Tot slice
 = ({ base = b; len = len; })
 
 let wvalid_stable
   (#k: parser_kind)
   (#t: Type)
   (p: parser k t)
-  (s: fslice)
+  (s: slice)
   (pos: U32.t)
   (gpos' : Ghost.erased U32.t)
   (v' : Ghost.erased t)
 : Lemma
   (requires (k.parser_kind_subkind == Some ParserStrong))
   (ensures (
-    stable_on (wvalid p s (compl t) pos gpos' v') freezable_preorder
+    stable_on (wvalid p s (compl t) pos gpos' v') prefix_freezable_preorder
   ))
 = let pf (s1 s2: Seq.seq byte) : Lemma
-    (requires (wvalid p s (compl t) pos gpos' v' s1 /\ freezable_preorder s1 s2))
-    (ensures (wvalid p s (compl t) pos gpos' v' s1 /\ freezable_preorder s1 s2 /\ wvalid p s (compl t) pos gpos' v' s2))
-  = parse_strong_prefix p (Seq.slice s1 (U32.v pos) (U32.v s.len)) (Seq.slice s2 (U32.v pos) (U32.v s.len))
+    (requires (wvalid p s (compl t) pos gpos' v' s1 /\ prefix_freezable_preorder s1 s2))
+    (ensures (wvalid p s (compl t) pos gpos' v' s1 /\ prefix_freezable_preorder s1 s2 /\ wvalid p s (compl t) pos gpos' v' s2))
+  = prefix_freezable_preorder_elim s1 s2;
+    parse_strong_prefix p (Seq.slice s1 (U32.v pos) (U32.v s.len)) (Seq.slice s2 (U32.v pos) (U32.v s.len))
   in
   let pf' (s1 s2: Seq.seq byte) : Lemma
-    ((wvalid p s (compl t) pos gpos' v' s1 /\ freezable_preorder s1 s2) ==> wvalid p s (compl t) pos gpos' v' s2)
+    ((wvalid p s (compl t) pos gpos' v' s1 /\ prefix_freezable_preorder s1 s2) ==> wvalid p s (compl t) pos gpos' v' s2)
   = Classical.move_requires (pf s1) s2
   in
   Classical.forall_intro_2 pf'
@@ -64,11 +65,11 @@ let irepr
   (#t: Type)
   (#k: parser_kind)
   (p: parser k t)
-  (s: fslice)
+  (s: slice)
 = irepr p s (compl t)
 
-let frozen_until (buf: fbuffer) (h:HS.mem) : GTot nat =
-  get_w (B.as_seq h buf)
+let buffer_frozen_until (buf: buffer) (h:HS.mem) : GTot nat =
+  frozen_until (B.as_seq h buf)
 
 inline_for_extraction
 noextract
@@ -76,7 +77,7 @@ let witness_valid
   (#t: Type)
   (#k: parser_kind)
   (#p: parser k t)
-  (s: fslice)
+  (s: slice)
   (pos: U32.t)
 : HST.Stack (irepr p s)
   (requires (fun h ->
@@ -84,7 +85,7 @@ let witness_valid
     valid p h s pos /\
     (* conditions on global size header *)
     U32.v pos >= 4 /\ (
-    let len = frozen_until s.base h in
+    let len = buffer_frozen_until s.base h in
     U32.v (get_valid_pos p h s pos) <= len
   )))
   (ensures (fun h res h' ->
@@ -93,7 +94,7 @@ let witness_valid
     valid_content_pos p h s pos (irepr_v res) (irepr_pos' res)
   ))
 = let h = HST.get () in
-  recall_w_default s.base;
+  recall_frozen_until_default s.base;
   wvalid_stable p s pos (Ghost.hide (get_valid_pos p h s pos)) (Ghost.hide (contents p h s pos));
   witness_valid_gen s (compl t) pos
 
@@ -103,7 +104,7 @@ let recall_valid
   (#t: Type)
   (#k: parser_kind)
   (#p: parser k t)
-  (#s: fslice)
+  (#s: slice)
   (i: irepr p s)
 : HST.Stack unit
   (requires (fun h -> B.recallable s.base \/ live_slice h s))
@@ -113,7 +114,7 @@ let recall_valid
     valid_content_pos p h s (irepr_pos i) (irepr_v i) (irepr_pos' i) /\
     U32.v s.len >= 4 /\
     U32.v (irepr_pos i) >= 4 /\
-    U32.v (irepr_pos' i) <= frozen_until s.base h
+    U32.v (irepr_pos' i) <= buffer_frozen_until s.base h
   ))
 = recall_valid_gen i
 
@@ -129,7 +130,7 @@ let iaccess
   (#cl: clens t1 t2)
   (#g: gaccessor p1 p2 cl)
   ($a: accessor g)
-  (#s: fslice)
+  (#s: slice)
   (i1: irepr p1 s)
 : HST.Stack (irepr p2 s)
   (requires (fun h ->
@@ -147,7 +148,7 @@ let iaccess
   ))
 = recall_valid i1;
   let x = a s (irepr_pos i1) in
-  recall_w_default s.base;
+  recall_frozen_until_default s.base;
   witness_valid s x
 
 inline_for_extraction
@@ -157,7 +158,7 @@ let iread
   (#t: Type)
   (#p: parser k t)
   (r: leaf_reader p)
-  (#s: fslice)
+  (#s: slice)
   (i: irepr p s)
 : HST.Stack t
   (requires (fun h -> (B.recallable s.base \/ live_slice h s)))
@@ -175,7 +176,7 @@ let ijump
   (#t: Type)
   (#p: parser k t)
   (j: jumper p)
-  (#s: fslice)
+  (#s: slice)
   (i: irepr p s)
 : HST.Stack U32.t
   (requires (fun h -> (B.recallable s.base \/ live_slice h s)))
@@ -188,12 +189,12 @@ let ijump
   j s (irepr_pos i)
 
 let freezable_buffer_writable_intro
-  (b: fbuffer)
+  (b: buffer)
   (pos pos' : nat)
   (h: HS.mem)
 : Lemma
   (requires (
-    let len = frozen_until b h in
+    let len = buffer_frozen_until b h in
     B.live h b /\
     4 <= len /\
     len <= pos
@@ -204,6 +205,7 @@ let freezable_buffer_writable_intro
   then
     let s = B.as_seq h b in
     let slen = Seq.slice s 0 4 in
+    Classical.forall_intro_2 prefix_freezable_preorder_elim;
     writable_intro b pos pos' h () (fun s1 s2 ->
       assert (Seq.slice (Seq.replace_subseq s pos pos' s1) 0 4 `Seq.equal` slen);
       assert (Seq.slice (Seq.replace_subseq s pos pos' s2) 0 4 `Seq.equal` slen)
@@ -215,25 +217,25 @@ let freeze_valid
   (#k: parser_kind)
   (#t: Type)
   (p: parser k t)
-  (sl: fslice)
+  (sl: slice)
   (pos: U32.t)
   (pos' : U32.t)
 : HST.Stack (irepr p sl)
   (requires (fun h ->
     (B.recallable sl.base \/ live_slice h sl) /\
-    frozen_until sl.base h <= U32.v pos /\
+    buffer_frozen_until sl.base h <= U32.v pos /\
     valid_pos p h sl pos pos' /\
     U32.v pos' < U32.v sl.len /\ // TODO: remove once replaced with <= in FreezableBuffer
     k.parser_kind_subkind == Some ParserStrong // for valid_exact_ext_intro
   ))
   (ensures (fun h res h' ->
     B.modifies (B.loc_buffer sl.base) h h' /\
-    frozen_until sl.base h' == U32.v pos' /\
+    buffer_frozen_until sl.base h' == U32.v pos' /\
     irepr_pos res == pos /\
     irepr_pos' res == pos' /\
     irepr_v res == contents p h sl pos
   ))
-=    B.recall_p sl.base (w_pred 4); // to recover liveness
+=    B.recall_p sl.base (frozen_until_at_least 4); // to recover liveness
      let h1 = HST.get () in
      freeze sl.base pos' ;
      let h2 = HST.get () in
@@ -242,15 +244,15 @@ let freeze_valid
      witness_valid sl pos
 
 let frozen_until_frame
-  (sl: fslice)
+  (sl: slice)
   (l: B.loc)
   (h h' : HS.mem)
 : Lemma
   (requires (live_slice h sl /\ B.modifies l h h' /\ B.loc_disjoint l (loc_slice_from_to sl 0ul 4ul)))
-  (ensures (frozen_until sl.base h' == frozen_until sl.base h))
+  (ensures (buffer_frozen_until sl.base h' == buffer_frozen_until sl.base h))
   [SMTPatOr [
-    [SMTPat (B.modifies l h h'); SMTPat (frozen_until sl.base h);];
-    [SMTPat (B.modifies l h h'); SMTPat (frozen_until sl.base h');];
+    [SMTPat (B.modifies l h h'); SMTPat (buffer_frozen_until sl.base h);];
+    [SMTPat (B.modifies l h h'); SMTPat (buffer_frozen_until sl.base h');];
   ]]
 = loc_slice_from_to_eq sl 0ul 4ul;
   B.modifies_buffer_from_to_elim sl.base 0ul 4ul l h h'
@@ -264,12 +266,12 @@ let iwrite
   (#s: serializer p)
   (w: leaf_writer_strong s)
   (v: t)
-  (sl: fslice)
+  (sl: slice)
   (pos: U32.t)
 : HST.Stack (irepr p sl)
   (requires (fun h ->
     k.parser_kind_subkind == Some ParserStrong /\ // for valid_exact_ext_intro
-    frozen_until sl.base h <= U32.v pos /\
+    buffer_frozen_until sl.base h <= U32.v pos /\
     U32.v pos + serialized_length s v < U32.v sl.len /\ // TODO: change to <=
     (recallable sl.base \/ live_slice h sl)
   ))
@@ -277,10 +279,10 @@ let iwrite
     irepr_v i == v /\
     irepr_pos i == pos /\
     irepr_pos' i == pos `U32.add` U32.uint_to_t (serialized_length s v) /\
-    frozen_until sl.base h' == U32.v (irepr_pos' i) /\
+    buffer_frozen_until sl.base h' == U32.v (irepr_pos' i) /\
     B.modifies (B.loc_buffer sl.base) h h'
   ))
-=    B.recall_p sl.base (w_pred 4); // to recover liveness
+=    B.recall_p sl.base (frozen_until_at_least 4); // to recover liveness
      let pos' = w v sl pos in
      freeze_valid p sl pos pos'
 
