src/lowparse/TestPair.fst
@@ -1,15 +1,15 @@
 module TestPair
 module P = Pair
-open LowParse.MLow
 module U8 = FStar.UInt8
-module FB = LowStar.FreezableBuffer
+module FB = LowStar.PrefixFreezableBuffer
 module LM = LowParseExampleMono
+module LMI = LowParse.MLow.Int
 
 assume val buf :
-  s: LM.fslice{
-    FB.recallable s.base
+  s: LM.slice{
+    FB.recallable s.LM.base
   }
-let irepr #t #k (p:parser k t) = LM.irepr p buf
+let irepr #t #k (p:LM.parser k t) = LM.irepr p buf
 
 module LPI = LowParse.Spec.AllIntegers
 
@@ -23,20 +23,13 @@ let read_components (i:irepr P.pair_parser)
     (ensures fun h0 x h1 ->
       True)
   = LM.recall_valid i;
-    let x = P.accessor_pair_fst buf (IRepr?.pos i) in
+    let x = P.accessor_pair_fst buf (LM.irepr_pos i) in
     havoc();
     LM.recall_valid i;
-    let y : UInt32.t = P.accessor_pair_snd buf (IRepr?.pos i) in
+    let y : UInt32.t = P.accessor_pair_snd buf (LM.irepr_pos i) in
     x, y
 
 module B = LowStar.Buffer
-// assume val frozen_until (f:FB.fbuffer)
-//   : Stack UInt32.t
-//     (requires fun h ->
-//       FB.recallable f \/ B.live h f)
-//     (ensures fun h0 x h1 ->
-//       h0 == h1 /\
-//       FB.get_w (B.as_seq h0 f) == UInt32.v x)
 
 let read_components2 (i:irepr P.pair_parser)
   : Stack (x: (irepr LPI.parse_u32 * irepr LPI.parse_u16) { LM.irepr_v i == {P.fst = LM.irepr_v (fst x); P.snd = LM.irepr_v (snd x)} } )
@@ -45,15 +38,15 @@ let read_components2 (i:irepr P.pair_parser)
     (ensures fun h0 x h1 ->
       True)
   = LM.recall_valid i;
-    let x = P.accessor_pair_fst buf (IRepr?.pos i) in
-    FB.recall_w_default buf.base;
+    let x = P.accessor_pair_fst buf (LM.irepr_pos i) in
+    FB.recall_frozen_until_default buf.LM.base;
     let x : irepr LPI.parse_u32 = LM.witness_valid buf x in
 
     havoc();
 
     LM.recall_valid i;
-    let y : UInt32.t = P.accessor_pair_snd buf (IRepr?.pos i) in
-    FB.recall_w_default buf.base;
+    let y : UInt32.t = P.accessor_pair_snd buf (LM.irepr_pos i) in
+    FB.recall_frozen_until_default buf.LM.base;
     assert (UInt32.v y >= 4);
     let y : irepr LPI.parse_u16 = LM.witness_valid buf y in
     x, y
@@ -72,31 +65,29 @@ let read_components3 (i:irepr P.pair_parser)
 module HS = FStar.HyperStack
 module U32 = FStar.UInt32
 
-let frozen_until = LM.frozen_until buf.base
-
-module LMI = LowParse.MLow.Int
+let frozen_until = LM.buffer_frozen_until buf.LM.base
 
 let iwrite_u16 (u:UInt16.t) (p:UInt32.t)
   : Stack (irepr LPI.parse_u16)
     (requires fun h ->
       frozen_until h <= U32.v p /\
-      U32.v p + 2 < U32.v buf.len)
+      U32.v p + 2 < U32.v buf.LM.len)
     (ensures fun h0 i h1 ->
       LM.irepr_pos i == p /\
       LM.irepr_pos' i == U32.(p +^ 2ul) /\
       LM.irepr_v i == u   /\
       frozen_until h1 == U32.v p + 2 /\
-      B.modifies (B.loc_buffer buf.base) h0 h1)
-   = FB.recall_w_default buf.base;
-     B.recall buf.base;
+      B.modifies (B.loc_buffer buf.LM.base) h0 h1)
+   = FB.recall_frozen_until_default buf.LM.base;
+     B.recall buf.LM.base;
      let h0 = get () in
      let p' = LMI.write_u16 u buf p in
      LM.loc_slice_from_to_eq buf 0ul 4ul;
      let h1 = get () in
      let p' = p `U32.add` 2ul in
-     B.modifies_buffer_from_to_elim buf.base 0ul 4ul (LM.loc_slice_from_to buf p p') h0 h1;
-     FB.recall_w_default buf.base;
-     FB.freeze buf.base p' ;
+     B.modifies_buffer_from_to_elim buf.LM.base 0ul 4ul (LM.loc_slice_from_to buf p p') h0 h1;
+     FB.recall_frozen_until_default buf.LM.base;
+     FB.freeze buf.LM.base p' ;
      let h2 = get () in
      LM.valid_exact_ext_intro LPI.parse_u16 h1 buf p p' h2 buf p p' ;
      LM.witness_valid buf p
@@ -106,23 +97,23 @@ let iwrite_u32 (u:UInt32.t) (p:UInt32.t)
   : Stack (irepr LPI.parse_u32)
     (requires fun h ->
       frozen_until h <= U32.v p /\
-      U32.v p + 4 < U32.v buf.len)
+      U32.v p + 4 < U32.v buf.LM.len)
     (ensures fun h0 i h1 ->
       LM.irepr_pos i == p /\
       LM.irepr_pos' i == U32.(p +^ 4ul) /\
       LM.irepr_v i == u   /\
       frozen_until h1 == U32.v p + 4 /\
-      B.modifies (B.loc_buffer buf.base) h0 h1)
-   = FB.recall_w_default buf.base;
-     B.recall buf.base;
+      B.modifies (B.loc_buffer buf.LM.base) h0 h1)
+   = FB.recall_frozen_until_default buf.LM.base;
+     B.recall buf.LM.base;
      let h0 = get () in
      let p' = LMI.write_u32 u buf p in
      LM.loc_slice_from_to_eq buf 0ul 4ul;
      let h1 = get () in
      let p' = p `U32.add` 4ul in
-     B.modifies_buffer_from_to_elim buf.base 0ul 4ul (LM.loc_slice_from_to buf p p') h0 h1;
-     FB.recall_w_default buf.base;
-     FB.freeze buf.base p' ;
+     B.modifies_buffer_from_to_elim buf.LM.base 0ul 4ul (LM.loc_slice_from_to buf p p') h0 h1;
+     FB.recall_frozen_until_default buf.LM.base;
+     FB.freeze buf.LM.base p' ;
      let h2 = get () in
      LM.valid_exact_ext_intro LPI.parse_u32 h1 buf p p' h2 buf p p' ;
      LM.witness_valid buf p
@@ -138,13 +129,13 @@ let iwrite_pair (u0:UInt32.t) (u1:UInt16.t) (p:UInt32.t)
   : Stack (irepr P.pair_parser)
     (requires fun h ->
       frozen_until h <= U32.v p /\
-      U32.v p + 6 < U32.v buf.len)
+      U32.v p + 6 < U32.v buf.LM.len)
     (ensures fun h0 i h1 ->
       LM.irepr_pos i == p /\
       LM.irepr_pos' i == U32.(p +^ 6ul) /\
       LM.irepr_v i == P.({fst=u0; snd=u1})  /\
       frozen_until h1 == U32.v p + 6 /\
-      B.modifies (B.loc_union some_loc (B.loc_buffer buf.base)) h0 h1)
+      B.modifies (B.loc_union some_loc (B.loc_buffer buf.LM.base)) h0 h1)
    = let i0 = iwrite_u32 u0 p in
      havoc_l some_loc;
      let i1 = iwrite_u16 u1 U32.(p +^ 4ul) in
@@ -160,16 +151,16 @@ let iwrite_pair1 (u0:UInt32.t) (u1:UInt16.t) (p:UInt32.t)
   : Stack (irepr P.pair_parser)
     (requires fun h ->
       frozen_until h <= U32.v p /\
-      U32.v p + 6 < U32.v buf.len)
+      U32.v p + 6 < U32.v buf.LM.len)
     (ensures fun h0 i h1 ->
       LM.irepr_pos i == p /\
       LM.irepr_pos' i == U32.(p +^ 6ul) /\
       LM.irepr_v i == P.({fst=u0; snd=u1})  /\
       frozen_until h1 == U32.v p + 6 /\
-      B.modifies (B.loc_union some_loc (B.loc_buffer buf.base)) h0 h1)
-   = let i0 = LM.iwrite write_u32 u0 buf p in
+      B.modifies (B.loc_union some_loc (B.loc_buffer buf.LM.base)) h0 h1)
+   = let i0 = LM.iwrite LMI.write_u32 u0 buf p in
      havoc_l some_loc;
-     let i1 = LM.iwrite write_u16 u1 buf U32.(p +^ 4ul) in
+     let i1 = LM.iwrite LMI.write_u16 u1 buf U32.(p +^ 4ul) in
      let h = get () in
      LM.recall_valid i0;
      LM.recall_valid i1;
@@ -182,17 +173,17 @@ let iwrite_pair2 (u0:UInt32.t) (u1:UInt16.t) (p:UInt32.t)
   : Stack (irepr P.pair_parser)
     (requires fun h ->
       frozen_until h <= U32.v p /\
-      U32.v p + 6 < U32.v buf.len)
+      U32.v p + 6 < U32.v buf.LM.len)
     (ensures fun h0 i h1 ->
       LM.irepr_pos i == p /\
       LM.irepr_pos' i == U32.(p +^ 6ul) /\
       LM.irepr_v i == P.({fst=u0; snd=u1})  /\
       frozen_until h1 == U32.v p + 6 /\
-      B.modifies (B.loc_union some_loc (B.loc_buffer buf.base)) h0 h1)
-= FB.recall_w_default buf.base; // for writable
-  B.recall buf.base; // for live
-  let p1 = write_u32 u0 buf p in
-  let p2 = write_u16 u1 buf p1 in
+      B.modifies (B.loc_union some_loc (B.loc_buffer buf.LM.base)) h0 h1)
+= FB.recall_frozen_until_default buf.LM.base; // for writable
+  B.recall buf.LM.base; // for live
+  let p1 = LMI.write_u32 u0 buf p in
+  let p2 = LMI.write_u16 u1 buf p1 in
   let h = get () in
   Pair.pair_valid h buf p;
   LM.freeze_valid Pair.pair_parser buf p p2
